Setting up for finishing the main result.

concurrency/Clight_new2core.v
@@ -1,4 +1,7 @@
+Require Import compcert.common.Values.
+
 Require Import concurrency.machine_simulation.
+Require Import concurrency.permissions.
 
 Require Import concurrency.DryMachineSource.
 Require Import concurrency.DryMachineSourceCore.
@@ -29,7 +32,7 @@ Require Import concurrency.concursim_safety.
   Module Clight_new2core_simulation_safety:=
     concure_simulation_safety NewMachine CoreMachine.
 
-  Definition new2core_safe:
+  Theorem new2core_safe:
     forall (Sds : THE_DRY_MACHINE_SOURCE.DMS.FineConc.machine_state) 
          (Sm : Memory.Mem.mem) (Tds : DMS.FineConc.machine_state) 
          (Tm : Memory.Mem.mem) (cd : MSdata Values.Vundef new2core_simulation)
@@ -40,10 +43,30 @@ Require Import concurrency.concursim_safety.
         NewMachine.DryConc.safe_new_step gs (sch, nil, Sds) Sm) ->
        forall sch : DMS.SC.Sch,
        CoreMachine.DryConc.valid (sch, nil, Tds) ->
-       CoreMachine.DryConc.safe_new_step gt (sch, nil, Tds) Tm:=
-    Clight_new2core_simulation_safety.safety_preservation
-  gs gt sch psrc ptgt new2core_simulation.
+       CoreMachine.DryConc.safe_new_step gt (sch, nil, Tds) Tm.
+    exact (Clight_new2core_simulation_safety.safety_preservation
+  gs gt sch psrc ptgt new2core_simulation).
+  Qed.
 
+  Require Import compcert.common.Globalenvs.
+  Require Import compcert.lib.Integers.
+    Lemma Initial_dry_safety_concur:
+      forall (prog : Clight.program  )
+        (U : SCH.schedule) (n : nat) (b: block) init_m,
+        Genv.find_symbol (Clight_sim.CC.genv_genv(Clight.globalenv prog)) (Ctypes.prog_main prog) =
+        Some b ->
+        (Genv.init_mem (Ctypes.program_of_program prog)) = Some init_m ->
+      exists init_st,
+        (machine_semantics.initial_machine
+           (CoreDryConc.new_MachineSemantics U (Some (getCurPerm init_m, empty_map)))) (Clight.globalenv prog)
+                                                                                       init_m (Vptr b Int.zero) nil =
+        Some (init_st, None) /\
+        forall U',
+          CoreDryConc.new_valid (CoreDryConc.mk_nstate (U', nil, init_st) init_m) U' ->
+       CoreMachine.DryConc.safe_new_step_bound (Clight.globalenv prog) (U', nil, init_st)
+         init_m.
+    Proof.
+    Admitted.
   (*TODO: Get the Clight_new safety from Clight_safety.v and put it 
     together with the new2core_safe*)
   
