concurrency/HybridMachine_simulation_proof.v
@@ -262,7 +262,7 @@ Section OneThreadCompiledMatch.
       match_thread_compiled cd j (Kinit v1 v1') m1
                             (Kinit v2 v2') m2.
 
-  Record concur_match (cd: compiler_index)
+  Record concur_match (ocd: option compiler_index)
        (j:meminj) (cstate1: C1) (m1: mem) (cstate2: C2) (m2: mem):=
   { same_length: num_threads cstate1 = num_threads cstate2
     ; memcompat1: HybridMachine.mem_compatible _ _ _ cstate1 m1
@@ -289,6 +289,7 @@ Section OneThreadCompiledMatch.
         forall (i:nat),
           (i = hb')%nat ->
           forall (cnti1: containsThread cstate1 i),
+            exists cd, ocd = Some cd /\
           match_thread_compiled cd j
                                 (getThreadC cnti1)
                                 (restrPermMap (memcompat1 i cnti1).1)
@@ -320,11 +321,13 @@ Qed.
 End OneThreadCompiledMatch.
 
 Arguments same_length_contains {ms1 ms2}.
-Arguments memcompat1 {cd j cstate1 m1 cstate2 m2}.
-Arguments memcompat2 {cd j cstate1 m1 cstate2 m2}.
+Arguments memcompat1 {ocd j cstate1 m1 cstate2 m2}.
+Arguments memcompat2 {ocd j cstate1 m1 cstate2 m2}.
     
   Section HybridThreadDiagram.
     Notation the_simulation := compiler_simulation.
+
+    Parameter option_compiler_order: option (Injindex the_simulation) -> option (Injindex the_simulation) -> Prop.
     
     Lemma hybrid_thread_diagram:
       forall (U0 : list nat) (st1 : C1) (m1 : mem) (st1' : C1) (m1' : mem),
@@ -337,7 +340,7 @@ Arguments memcompat2 {cd j cstate1 m1 cstate2 m2}.
                (HCSem Sems Semt hb2 U) genv U0 st2 m2 st2' m2' \/
              machine_semantics_lemmas.thread_step_star
                (HCSem Sems Semt hb2 U) genv U0 st2 m2 st2' m2'
-             /\ compiler_order cd' cd).
+             /\ option_compiler_order cd' cd).
     Proof.
       intros.
       destruct U0; simpl in H.
@@ -432,7 +435,7 @@ Arguments memcompat2 {cd j cstate1 m1 cstate2 m2}.
           eapply H0 in EQ. instantiate (1 := Htid) in EQ.
           rewrite Hcode in EQ.
           assert (Htid':= contains12 H0 Htid).
-          inv EQ.
+          destruct EQ as [cd0 [cd_eq EQ]]; inv EQ.
           destruct H6 as (st1_ & m1_ & st2_ & m2_ &
                           f1 & f2 & f3 &
                           INJsrc & INJcomp & INJtgt &
@@ -522,9 +525,9 @@ Arguments memcompat2 {cd j cstate1 m1 cstate2 m2}.
     (m1 : mem) (U' : seq.seq nat) (tr' : seq.seq machine_event) (st1' : C1) 
     (m1' : mem),
   machine_semantics.machine_step (HCSem Sems Semt hb1 U) genv U0 tr st1 m1 U' tr' st1' m1' ->
-  forall (cd : Injindex compiler_simulation) (st2 : C2) (mu : meminj) (m2 : mem),
+  forall (cd : option (Injindex compiler_simulation)) (st2 : C2) (mu : meminj) (m2 : mem),
   concur_match cd mu st1 m1 st2 m2 ->
-  exists (st2' : C2) (m2' : mem) (cd' : Injindex compiler_simulation),
+  exists (st2' : C2) (m2' : mem) (cd' : option (Injindex compiler_simulation)),
     concur_match cd' mu st1' m1' st2' m2' /\
     machine_semantics.machine_step (HCSem Sems Semt hb2 U) genv U0 tr st2 m2 U' tr' st2' m2'.
     Proof.
@@ -551,6 +554,7 @@ Arguments memcompat2 {cd j cstate1 m1 cstate2 m2}.
           destruct (Compare_dec.lt_eq_lt_dec (tid) hb') as [[HH | HH] | HH ];
             (*In all cases discard non-running threads*)
             eapply H0 in HH; instantiate (1:= ctn) in HH;
+              try (destruct HH as [cd' [cd_eq HH]]);
               inv HH;  rewrite Hcode in H; inv H.
           (*then instantitates the same thing*)
           * exists (updThreadC_ (ThreadPool hb2 Sems Semt) ctn' (Kblocked (TState ClightCoreSEM.C Asm.regset code2))), m2, cd; split.
@@ -560,7 +564,7 @@ Arguments memcompat2 {cd j cstate1 m1 cstate2 m2}.
             econstructor; eauto.
             admit. (* should follow from the simulations *)
             admit. (* Add this to the match? *)
-          * exists (updThreadC_ (ThreadPool hb2 Sems Semt) ctn' (Kblocked (TState ClightCoreSEM.C Asm.regset code2))), m2, cd; split.
+          * exists (updThreadC_ (ThreadPool hb2 Sems Semt) ctn' (Kblocked (TState ClightCoreSEM.C Asm.regset code2))), m2, ( some cd'); split.
             admit. (*reestablish the match (should be easy*)
             econstructor; eauto.
             admit. (* Add this to the match*)
@@ -576,62 +580,62 @@ Arguments memcompat2 {cd j cstate1 m1 cstate2 m2}.
             admit. (* Add this to the match? *)
         + (*sync*)
           inv Htstep.
-          inv HschedN.
           (*LOCK*)
-         Lemma Lock_HybridStep_simulation:
-           forall (U0 : seq.seq nat)
-             (st1 : t Resources (Sem hb1 Sems Semt))
-             (m1 m1' : mem)
-  (cd : Injindex compiler_simulation)
-  (st2 : t Resources (Sem hb2 Sems Semt))
-  (mu : meminj)
-  (m2 : mem)
-  (H0 : concur_match cd mu st1 m1 st2 m2)
-  (tid : nat)
-  (Htid : containsThread st1 tid)
-  (Hcmpt : HybridMachine.mem_compatible hb1 Sems Semt st1 m1)
-  (c : state_sum ClightCoreSEM.C X86Machines.ErasedMachine.ThreadPool.code)
-  (b : block)
-  (ofs : Integers.Int.int)
-  (pmap : access_map * access_map)
-  (virtueThread : delta_map * delta_map),
-  let newThreadPerm := (computeMap (getThreadR Htid)#1 virtueThread#1,
-                   computeMap (getThreadR Htid)#2 virtueThread#2) : 
-               access_map * access_map in
-  forall (Hlt' : permMapLt
-           (setPermBlock (Some Writable) b (Integers.Int.intval ofs)
-              (getThreadR_ (ThreadPool hb1 Sems Semt) Htid)#2 LKSIZE_nat) 
-           (getMaxPerm m1))
-  (Hbounded : bounded_maps.sub_map virtueThread#1
-               (PTree.map1 (fun f : Z -> perm_kind -> option permission => f^~ Max)
-                  (Mem.mem_access m1)#2) /\
-             bounded_maps.sub_map virtueThread#2
-               (PTree.map1 (fun f : Z -> perm_kind -> option permission => f^~ Max)
-                  (Mem.mem_access m1)#2))
-  (Hinv : HybridMachine.invariant hb1 Sems Semt st1)
-  (Hcode : getThreadC Htid = Kblocked c)
-  (Hat_external : at_external_sum ClightCoreSEM.G X86SEM.G ClightCoreSEM.C
-                   X86Machines.ErasedMachine.ThreadPool.code mem
-                   (semantics.at_external
-                      (semantics.csem (event_semantics.msem ClightCoreSEM.Sem)))
-                   Asm_core.cl_at_external genv c m1 = Some (LOCK, [:: Vptr b ofs]))
-  (Hload : Mem.load Mint32 (restrPermMap (proj2 (Hcmpt tid Htid))) b (Integers.Int.intval ofs) =
-          Some (Vint Integers.Int.one))
-  (Haccess : Mem.range_perm (restrPermMap (proj2 (Hcmpt tid Htid))) b 
-              (Integers.Int.intval ofs) (Integers.Int.intval ofs + LKSIZE) Cur Readable)
-  (Hstore : Mem.store Mint32 (restrPermMap Hlt') b (Integers.Int.intval ofs)
-             (Vint Integers.Int.zero) = Some m1')
-  (HisLock : lockRes st1 (b, Integers.Int.intval ofs) = Some pmap)
-  (Hangel1 : permMapJoin pmap#1 (getThreadR Htid)#1
-              (computeMap (getThreadR Htid)#1 virtueThread#1))
-  (Hangel2 : permMapJoin pmap#2 (getThreadR Htid)#2
-              (computeMap (getThreadR Htid)#2 virtueThread#2)),
-  exists
-    (st2' : t Resources (Sem hb2 Sems Semt)) (m2' : mem) (cd' : Injindex compiler_simulation),
-    concur_match cd' mu
-      (updLockSet (updThread Htid (Kresume c Vundef) newThreadPerm)
-         (b, Integers.Int.intval ofs) (empty_map, empty_map)) m1' st2' m2' /\
-    HybridMachine.external_step hb2 Sems Semt genv (tid :: U0) [::] st2 m2 U0 [::] st2' m2'.
+          * inv HschedN.
+            Lemma Lock_HybridStep_simulation:
+              forall (U0 : seq.seq nat)
+                (st1 : t Resources (Sem hb1 Sems Semt))
+                (m1 m1' : mem)
+                (cd : option (Injindex compiler_simulation))
+                (st2 : t Resources (Sem hb2 Sems Semt))
+                (mu : meminj)
+                (m2 : mem)
+                (H0 : concur_match cd mu st1 m1 st2 m2)
+                (tid : nat)
+                (Htid : containsThread st1 tid)
+                (Hcmpt : HybridMachine.mem_compatible hb1 Sems Semt st1 m1)
+                (c : state_sum ClightCoreSEM.C X86Machines.ErasedMachine.ThreadPool.code)
+                (b : block)
+                (ofs : Integers.Int.int)
+                (pmap : access_map * access_map)
+                (virtueThread : delta_map * delta_map),
+                let newThreadPerm := (computeMap (getThreadR Htid)#1 virtueThread#1,
+                                      computeMap (getThreadR Htid)#2 virtueThread#2) : 
+                                       access_map * access_map in
+                forall (Hlt' : permMapLt
+                            (setPermBlock (Some Writable) b (Integers.Int.intval ofs)
+                                          (getThreadR_ (ThreadPool hb1 Sems Semt) Htid)#2 LKSIZE_nat) 
+                            (getMaxPerm m1))
+                  (Hbounded : bounded_maps.sub_map virtueThread#1
+                                                   (PTree.map1 (fun f : Z -> perm_kind -> option permission => f^~ Max)
+                                                               (Mem.mem_access m1)#2) /\
+                              bounded_maps.sub_map virtueThread#2
+                                                   (PTree.map1 (fun f : Z -> perm_kind -> option permission => f^~ Max)
+                                                               (Mem.mem_access m1)#2))
+                  (Hinv : HybridMachine.invariant hb1 Sems Semt st1)
+                  (Hcode : getThreadC Htid = Kblocked c)
+                  (Hat_external : at_external_sum ClightCoreSEM.G X86SEM.G ClightCoreSEM.C
+                                                  X86Machines.ErasedMachine.ThreadPool.code mem
+                                                  (semantics.at_external
+                                                     (semantics.csem (event_semantics.msem ClightCoreSEM.Sem)))
+                                                  Asm_core.cl_at_external genv c m1 = Some (LOCK, [:: Vptr b ofs]))
+                  (Hload : Mem.load Mint32 (restrPermMap (proj2 (Hcmpt tid Htid))) b (Integers.Int.intval ofs) =
+                           Some (Vint Integers.Int.one))
+                  (Haccess : Mem.range_perm (restrPermMap (proj2 (Hcmpt tid Htid))) b 
+                                            (Integers.Int.intval ofs) (Integers.Int.intval ofs + LKSIZE) Cur Readable)
+                  (Hstore : Mem.store Mint32 (restrPermMap Hlt') b (Integers.Int.intval ofs)
+                                      (Vint Integers.Int.zero) = Some m1')
+                  (HisLock : lockRes st1 (b, Integers.Int.intval ofs) = Some pmap)
+                  (Hangel1 : permMapJoin pmap#1 (getThreadR Htid)#1
+                                         (computeMap (getThreadR Htid)#1 virtueThread#1))
+                  (Hangel2 : permMapJoin pmap#2 (getThreadR Htid)#2
+                                         (computeMap (getThreadR Htid)#2 virtueThread#2)),
+                exists
+                  (st2' : t Resources (Sem hb2 Sems Semt)) (m2' : mem) (cd' : option (Injindex compiler_simulation)),
+                  concur_match cd' mu
+                               (updLockSet (updThread Htid (Kresume c Vundef) newThreadPerm)
+                                           (b, Integers.Int.intval ofs) (empty_map, empty_map)) m1' st2' m2' /\
+                  HybridMachine.external_step hb2 Sems Semt genv (tid :: U0) [::] st2 m2 U0 [::] st2' m2'.
          Proof.
            intros.
            (*Steps:*)
@@ -662,8 +666,7 @@ Arguments memcompat2 {cd j cstate1 m1 cstate2 m2}.
              ).
              do 2 eexists; econstructor.
              simpl.
-             
-
+(*
              (*tid < hb' Noth threads on taret*) 
              (*Prove the comcert external_call step for thread i*)
              eapply H0 in LT. instantiate (1:= Htid) in LT; inv LT;
@@ -687,17 +690,18 @@ Arguments memcompat2 {cd j cstate1 m1 cstate2 m2}.
            (*Use the simulation to propagate it down.*)
            (*Use the machine step in the target machine, *)
            (* From the Comcert step, get the match*)
-
+            *)
            
            
          Admitted.
          eapply Lock_HybridStep_simulation; eauto.
-         admit.
+
+         * admit. * admit.  * admit.  * admit.  * admit.  
         + (*haltd*)
           admit.
         + (*schedfail'*)
           admit.
-    Admitted. *)
+    Admitted. 
     
   End MachineThreadDiagram.
 
@@ -707,25 +711,31 @@ Arguments memcompat2 {cd j cstate1 m1 cstate2 m2}.
     exists v:val,
             HybridMachine_simulation
               Sems Semt hb1 hb2 U genv
-              _ compiler_order
+              _ option_compiler_order
               (concur_match)  v.
   Proof.
     
   exists Vundef.
   econstructor.
-  - eapply Injfsim_order_wf.
+  - admit. (*eapply Injfsim_order_wf*)
   - (* core_initial*)
     intros.
-    (* intros.
-    simpl in H.
-    destruct (
-        HybridMachine.init_mach hb1 Sems Semt (@None (prod permissions.access_map permissions.access_map))
-            genv Vundef vals1
-      ) eqn:INIT; 
-    unfold HybridMachine.init_machine' in H;
-    rewrite INIT in H; inversion H; subst. (*solves one case*)
-    unfold HybridMachine.init_mach in INIT.  *)
-    admit.
+    destruct (NPeano.Nat.eq_dec hb' 0).
+    + pose proof (Injfsim_match_initial_states compiler_simulation).
+      unfold initial_state in H2; simpl in H2.
+      
+      
+
+      unfold Clight.initial_state in H2.
+      
+    + (*Easy case where the first thread is compiled already *)  exists None.
+      exists (mk _ (Sem hb2 Sems Semt) (num_threads c1) (pool c1) (perm_maps c1) (lset c1) ).
+      exists m1'.
+      split.
+      simpl in *; unfold HybridMachine.init_machine',
+                  HybridMachine.init_mach in *; simpl in *.
+      unfold initial_core_sum in *. admit. (*Could be lemma *)
+    
   - (*thread_diagram*)
     intros.
     eapply hybrid_thread_diagram; eauto.
